portage
git-svn-id: https://www.lri.fr/svn/demons/why2/trunk@1388 ecafba89-7d34-45a1-8a0b-92829e960b72

examples/bresenham/bresenham_why.v
@@ -18,7 +18,7 @@ Require Import ZArithRing.
 
 Axiom first_octant : (0 <= y2 <= x2)%Z.
 
-Ltac Omega' := generalize first_octant; omega.
+Ltac omega' := generalize first_octant; omega.
 
 (*s Specification of the correctness. 
     [(best x y)] expresses that the point [(x,y)] is the best
@@ -34,14 +34,14 @@ Definition best (x y:Z) :=
     [invariant_is_ok] establishes that this invariant implies the
     expected property. *)
 
-Definition invariant (x y e:Z) :=
+Definition Invariant (x y e:Z) :=
   e = (2 * (x + 1) * y2 - (2 * y + 1) * x2)%Z /\
   (2 * (y2 - x2) <= e <= 2 * y2)%Z.
 
-Lemma invariant_is_ok : forall x y e:Z, invariant x y e -> best x y.
+Lemma invariant_is_ok : forall x y e:Z, Invariant x y e -> best x y.
 Proof.
 intros x y e.
-unfold invariant; unfold best; intros [E I'] y'.
+unfold Invariant; unfold best; intros [E I'] y'.
 cut (0 <= x2)%Z; [ intro Hx2 | idtac ].
 apply closest.
 assumption.
@@ -67,48 +67,99 @@ Qed.
 
 (*s Program correctness. *)
 
-Proof.
-intros.
-decompose [and] Pre3.
-exact (invariant_is_ok x1 y1 e1 H0).
-Qed.
-
-Proof.
-intros.
-subst x.
-split.
- split.
- Omega'.
-unfold invariant.
- unfold invariant in Pre3.
-split.
-replace (2 * (x1 + 1 + 1) * y2)%Z with (2 * (x1 + 1) * y2 + 2 * y2)%Z;
- [ Omega' | ring ].
-Omega'.
-unfold Zwf; Omega'.
-Qed.
-
-Proof.
-intros.
-subst x.
-unfold invariant.
- unfold invariant in Pre3.
-split.
- split.
- Omega'.
-split.
- subst y3.
-replace (2 * (x1 + 1 + 1) * y2 - (2 * (y1 + 1) + 1) * x2)%Z with
- (2 * (x1 + 1) * y2 + 2 * y2 - (2 * y1 + 1) * x2 - 2 * x2)%Z;
- [ Omega' | ring ].
-Omega'.
-unfold Zwf; Omega'.
-Qed.
-
+(* Why obligation from file "", line 0, characters 0-0: *)
+(*Why goal*) Lemma bresenham_po_1 : 
+  forall (x: Z),
+  forall (HW_1: x = 0),
+  forall (y: Z),
+  forall (HW_2: y = 0),
+  forall (e: Z),
+  forall (HW_3: e = (2 * y2 - x2)),
+  (0 <= x /\ x <= (x2 + 1)) /\ (Invariant x y e).
 Proof.
 intuition.
-Omega'.
-subst x0; subst y0; subst e0; unfold invariant; Omega'.
-Qed.
+omega'.
+subst; unfold Invariant; omega'.
+Save.
 
+(* Why obligation from file "", line 0, characters 0-0: *)
+(*Why goal*) Lemma bresenham_po_2 : 
+  forall (x: Z),
+  forall (HW_1: x = 0),
+  forall (y: Z),
+  forall (HW_2: y = 0),
+  forall (e: Z),
+  forall (HW_3: e = (2 * y2 - x2)),
+  forall (HW_4: (0 <= x /\ x <= (x2 + 1)) /\ (Invariant x y e)),
+  forall (e0: Z),
+  forall (x0: Z),
+  forall (y0: Z),
+  forall (HW_5: (0 <= x0 /\ x0 <= (x2 + 1)) /\ (Invariant x0 y0 e0)),
+  forall (HW_6: x0 <= x2),
+  (best x0 y0).
+Proof.
+intuition.
+apply invariant_is_ok with e0; auto.
+Save.
+
+(* Why obligation from file "", line 0, characters 0-0: *)
+(*Why goal*) Lemma bresenham_po_3 : 
+  forall (x: Z),
+  forall (HW_1: x = 0),
+  forall (y: Z),
+  forall (HW_2: y = 0),
+  forall (e: Z),
+  forall (HW_3: e = (2 * y2 - x2)),
+  forall (HW_4: (0 <= x /\ x <= (x2 + 1)) /\ (Invariant x y e)),
+  forall (e0: Z),
+  forall (x0: Z),
+  forall (y0: Z),
+  forall (HW_5: (0 <= x0 /\ x0 <= (x2 + 1)) /\ (Invariant x0 y0 e0)),
+  forall (HW_6: x0 <= x2),
+  forall (HW_7: (best x0 y0)),
+  forall (HW_8: e0 < 0),
+  forall (e1: Z),
+  forall (HW_9: e1 = (e0 + 2 * y2)),
+  forall (x1: Z),
+  forall (HW_10: x1 = (x0 + 1)),
+  ((0 <= x1 /\ x1 <= (x2 + 1)) /\ (Invariant x1 y0 e1)) /\
+  (Zwf 0 (x2 + 1 - x1) (x2 + 1 - x0)).
+Proof.
+unfold Invariant; intuition; subst.
+replace (2 * (x0 + 1 + 1) * y2)%Z with (2 * (x0 + 1) * y2 + 2 * y2)%Z;
+ [ omega' | ring ].
+omega'.
+Save.
+
+(* Why obligation from file "", line 0, characters 0-0: *)
+(*Why goal*) Lemma bresenham_po_4 : 
+  forall (x: Z),
+  forall (HW_1: x = 0),
+  forall (y: Z),
+  forall (HW_2: y = 0),
+  forall (e: Z),
+  forall (HW_3: e = (2 * y2 - x2)),
+  forall (HW_4: (0 <= x /\ x <= (x2 + 1)) /\ (Invariant x y e)),
+  forall (e0: Z),
+  forall (x0: Z),
+  forall (y0: Z),
+  forall (HW_5: (0 <= x0 /\ x0 <= (x2 + 1)) /\ (Invariant x0 y0 e0)),
+  forall (HW_6: x0 <= x2),
+  forall (HW_7: (best x0 y0)),
+  forall (HW_11: e0 >= 0),
+  forall (y1: Z),
+  forall (HW_12: y1 = (y0 + 1)),
+  forall (e1: Z),
+  forall (HW_13: e1 = (e0 + 2 * (y2 - x2))),
+  forall (x1: Z),
+  forall (HW_14: x1 = (x0 + 1)),
+  ((0 <= x1 /\ x1 <= (x2 + 1)) /\ (Invariant x1 y1 e1)) /\
+  (Zwf 0 (x2 + 1 - x1) (x2 + 1 - x0)).
+Proof.
+unfold Invariant; intuition; subst.
+replace (2 * (x0 + 1 + 1) * y2 - (2 * (y0 + 1) + 1) * x2)%Z with
+ (2 * (x0 + 1) * y2 + 2 * y2 - (2 * y0 + 1) * x2 - 2 * x2)%Z;
+ [ omega' | ring ].
+omega'.
+Save.
 
